Make disk a sized, contiguous memory
Worked out surprisingly well, other than needing more accessor
functions.  Ironically the [D.State] record is still there and didn't
help make this change, so we only have more record accessors.

One annoyance remaining is that for disks it's now natural to test if
the address is in the domain by checking if it's less than the size, but
everywhere else we use the more general check on the disk memory itself.
Checking the memory is probably better but a bit awkward.

Currently we explicitly call [diskMem], which can be used for printing
but is not a disk >-> Funclass coercion so it can't be used to do [d a]
and access an address within a disk. We should probably use a coercion
to Funclass instead.

The code still doesn't know how big the disk is, but we could have a
parameter and assume it's correct in the theorem, or even add an
operation to get the disk size.

Disk.v
@@ -11,4 +11,89 @@ Definition block := bytes fourkilobytes.
 Definition block0 : block := bytes0 fourkilobytes.
 Opaque block.
 
-Definition disk := mem addr block.
+Record disk :=
+  mkDisk { size: nat;
+           diskMem :> mem addr block;
+           diskMem_domain: sized_domain diskMem size; }.
+
+(* this is an alternative to make fetching from a disk completely transparent *)
+Definition diskMem_fun (d:disk) : addr -> option block := diskMem d.
+Coercion diskMem_fun : disk >-> Funclass.
+
+Arguments mkDisk size diskMem diskMem_domain : clear implicits.
+
+Definition empty_disk : disk := mkDisk 0 empty_mem (sized_domain_empty _).
+
+Definition diskUpd (d: disk) (a: addr) (b: block) : disk.
+Proof.
+  destruct (lt_dec a (size d)).
+  - refine (mkDisk (size d) (upd d a b) _).
+    apply sized_domain_upd_lt; auto.
+    exact (diskMem_domain d).
+  - exact d.
+Defined.
+
+Lemma diskUpd_eq_some : forall d a b0 b,
+    diskMem d a = Some b0 ->
+    diskMem (diskUpd d a b) a = Some b.
+Proof.
+  intros.
+  pose proof (diskMem_domain d a).
+  unfold diskUpd.
+  destruct (lt_dec a (size d)); try contradiction; simpl.
+  autorewrite with upd; auto.
+  congruence.
+Qed.
+
+Lemma diskUpd_eq : forall d a b,
+    a < size d ->
+    diskMem (diskUpd d a b) a = Some b.
+Proof.
+  intros.
+  unfold diskUpd.
+  destruct (lt_dec a (size d)); try contradiction; simpl.
+  autorewrite with upd; auto.
+Qed.
+
+Lemma diskUpd_oob_eq : forall d a b,
+    ~a < size d ->
+    diskMem (diskUpd d a b) a = None.
+Proof.
+  intros.
+  unfold diskUpd.
+  pose proof (diskMem_domain d a).
+  destruct (lt_dec a (size d)); try contradiction; simpl; eauto.
+Qed.
+
+Lemma diskUpd_neq : forall d a b a',
+    a <> a' ->
+    diskMem (diskUpd d a b) a' = diskMem d a'.
+Proof.
+  intros.
+  unfold diskUpd.
+  destruct (lt_dec a (size d)); simpl;
+    autorewrite with upd; auto.
+Qed.
+
+Lemma diskUpd_size : forall d a b,
+    size (diskUpd d a b) = size d.
+Proof.
+  unfold diskUpd; intros.
+  destruct (lt_dec a (size d)); eauto.
+Qed.
+
+Lemma diskUpd_none : forall d a b,
+    diskMem d a = None ->
+    diskUpd d a b = d.
+Proof.
+  unfold diskUpd; intros.
+  pose proof (diskMem_domain d a).
+  destruct (lt_dec a (size d)); eauto.
+  destruct H0; congruence.
+Qed.
+
+Hint Rewrite diskUpd_eq using (solve [ auto ]) : upd.
+Hint Rewrite diskUpd_oob_eq using (solve [ auto ]) : upd.
+Hint Rewrite diskUpd_size : upd.
+Hint Rewrite diskUpd_neq using (solve [ auto ]) : upd.
+Hint Rewrite diskUpd_none using (solve [ auto ]) : upd.
