Mem.v
@@ -48,3 +48,42 @@ Definition empty_mem {A AEQ V} : @mem A AEQ V := fun _ => None.
 Hint Rewrite upd_eq : upd.
 Hint Rewrite upd_upd : upd.
 Hint Rewrite upd_neq using (solve [ auto ]) : upd.
+
+Definition lt_dec (a b:nat) : {a < b} + {~a < b}.
+Proof.
+  apply Compare_dec.lt_dec.
+Defined.
+
+Definition sized_domain V (m: mem nat V) sz :=
+  forall a, if lt_dec a sz then
+         exists v, m a = Some v
+       else m a = None.
+
+Theorem sized_domain_upd_some : forall V (m:mem nat V) sz a v0 v,
+    m a = Some v0 ->
+    sized_domain m sz ->
+    sized_domain (upd m a v) sz.
+Proof.
+  unfold sized_domain; intros.
+  specialize (H0 a0).
+  unfold upd.
+  destruct matches; repeat deex; eauto.
+Qed.
+
+Theorem sized_domain_upd_lt : forall V (m:mem nat V) sz a v,
+    a < sz ->
+    sized_domain m sz ->
+    sized_domain (upd m a v) sz.
+Proof.
+  unfold sized_domain; intros.
+  specialize (H0 a0).
+  unfold upd.
+  destruct matches; repeat deex; eauto.
+Qed.
+
+Theorem sized_domain_empty V : sized_domain (empty_mem (V:=V)) 0.
+Proof.
+  unfold sized_domain; intros.
+  destruct (lt_dec a 0); auto.
+  inversion l.
+Qed.
