Refinement/SeqDiskImpl.v
@@ -17,10 +17,7 @@ Module D.
     fun ds => DSpec.Disk (TDSpec.disk0 ds).
 
   Definition invariant (ds:TDSpec.State) :=
-    forall a, match TDSpec.disk0 ds a with
-         | Some v0 => exists v1, TDSpec.disk1 ds a = Some v1
-         | None => TDSpec.disk1 ds a = None
-         end.
+    size (TDSpec.disk0 ds) = size (TDSpec.disk1 ds).
 
   (* we need this lemma due to some terrible behavior in congruence:
    https://coq.inria.fr/bugs/show_bug.cgi?id=5394 *)
@@ -52,12 +49,10 @@ Module D.
 
   Lemma invariant_stable_upd : forall d_0 d_1 a b,
       invariant (TDSpec.Disks d_0 d_1) ->
-      invariant (TDSpec.Disks (upd d_0 a b) (upd d_1 a b)).
+      invariant (TDSpec.Disks (diskUpd d_0 a b) (diskUpd d_1 a b)).
   Proof.
     unfold invariant; simpl; intros.
-    destruct (a == a0); unfold equiv, complement in *; subst;
-      autorewrite with upd; eauto.
-    apply H.
+    autorewrite with upd; auto.
   Qed.
 
   Hint Resolve invariant_stable_upd.
@@ -77,18 +72,13 @@ Module D.
            | [ H: io_step (TD.Write _ _ _) _ _ _ |- _ ] =>
              eapply TD.Write_ok in H; simpl in H; safe_intuition
            end.
-    destruct matches; safe_intuition; subst;
-      hide_fn TD.abstraction;
-      match goal with
+    safe_intuition;
+      hide_fn TD.abstraction; subst;
+      try match goal with
       | [ H: invariant _ |- _ ] =>
         pose proof (H a); repeat (simpl_match || deex)
-      end.
-    - rewrite TDSpec.get_disk1_upd_d0 in *.
-      simpl_match; subst.
-      destruct t; simpl.
-      intuition eauto.
-    - repeat (subst || simpl_match).
-      intuition eauto.
+          end.
+    unfold TDSpec.upd_disk; destruct matches.
   Qed.
 
 End D.
