Refinement/SeqDiskAPI.v
@@ -1,5 +1,6 @@
 Require Export Disk.
 Require Import Implements.
+Require Import ProofIrrelevance.
 Require Import FunctionalExtensionality.
 
 Module DSpec.
@@ -7,27 +8,32 @@ Module DSpec.
     Disk { sdisk : disk }.
 
   Lemma state_eq : forall (state state':State),
-      (forall a, sdisk state a = sdisk state' a) ->
+      size (sdisk state) = size (sdisk state') ->
+      (forall a, diskMem (sdisk state) a = diskMem (sdisk state') a) ->
       state = state'.
   Proof.
     intros.
     destruct state, state'; simpl in *; f_equal.
-    extensionality a.
-    eauto.
+    destruct sdisk0, sdisk1.
+    simpl in *; subst.
+    assert (diskMem = diskMem0).
+    extensionality a; auto.
+    subst.
+    assert (diskMem_domain = diskMem_domain0).
+    apply proof_irrelevance.
+    subst.
+    auto.
   Qed.
 
   Definition Read a : Semantics block :=
     StepRel (fun state r state' =>
-               match sdisk state a with
+               match diskMem (sdisk state) a with
                | Some v0 => r = v0
                | None => True
                end /\ state' = state).
 
   Definition Write a b : Semantics unit :=
     StepRel (fun state r state' =>
-               match sdisk state a with
-               | Some v0 => state' = Disk (upd (sdisk state) a b)
-               | None => state' = state
-               end /\ r = tt).
+               state' = Disk (diskUpd (sdisk state) a b) /\ r = tt).
 
 End DSpec.
